Introduce concrete implementation of Map
Summary:
Replace the current implementation of `Map` (which using Coq functions)
with a more concrete one based on association lists. We gain a nice
extensionality property and type unicity which allows us not to depend
on any axiom while still enjoying some nice type structures.

Reviewed By: grievejia

Differential Revision: D18299892

fbshipit-source-id: 2371c966e7d752b6efc3c17d94d65751e1c5ec71

docs/formal/python_semantic/Map.v
@@ -1,32 +1,466 @@
-Require Import String List.
+Require Import Arith Ascii String List Sorted.
+Import ListNotations.
+Require Import Pyre.Lib.String Pyre.Lib.List.
 
-(** * Map *)
+(** In this module, we define the main <<State>> structure of our judgements.
+The underlying structure is a <<Map>> indexed by <<string>>s. They are
+implemented using lists of "key/value" pairs, strictly (no duplicated entries)
+sorted by keys. *)
 
+(* Some helper definitions to deal encapsulate/project the order on string to
+order of pairs of (string/anything). *)
+Section SortedListHelpers.
+Variable A: Type.
+
+(* Pair comparison by only using the first member *)
+Definition pair_ltb (elt0 elt1: string * A) : bool :=
+  ltb (fst elt0) (fst elt1)
+.
+
+(* Propositional equivalent of the boolean relation pair_ltb *)
+Definition pair_lt (elt0 elt1: string * A) : Prop :=
+  pair_ltb elt0 elt1 = true
+.
+
+(* begin hide *)
+Lemma HdRel_pair_lt_right: forall l key value0 value1,
+  HdRel pair_lt (key, value0) l -> HdRel pair_lt (key, value1) l.
+Proof.
+intros [ | hd tl] key v0 v1 h; simpl in *; [ now constructor | ].
+apply HdRel_inv in h; constructor.
+now unfold pair_lt in *.
+Qed.
+
+Lemma pair_lt_trans: forall (x y z: string * A),
+  pair_ltb x y = true -> pair_ltb y z = true -> pair_ltb x z = true.
+Proof.
+intros [x0 x1] [y0 y1] [z0 z1]; unfold pair_ltb; intros h0 h1; simpl in *.
+now apply ltb_trans with (y := y0).
+Qed.
+
+Lemma Forall_pair_lt: forall key1 value1 key2 value2,
+  pair_lt (key1, value1) (key2, value2) ->
+  forall l, Forall (pair_lt (key2, value2)) l ->
+  Forall (pair_lt (key1, value1)) l.
+Proof.
+intros key1 value1 key2 value2 hp.
+induction l as [ | [k v] l hi]; intros hf; simpl in *; [ now constructor | ].
+constructor.
+- eapply pair_lt_trans; [now apply hp| ].
+  now apply Forall_inv in hf.
+- apply hi.
+  now apply Forall_inv_tail in hf.
+Qed.
+(* end hide *)
+End SortedListHelpers.
+
+(** * Map
+
+A <<Map>> is a stricly sorted list of key/value pairs which helps keeping
+track of types / values in the rest of the developlment. *)
 Section Map.
+
+(* Generic type of values *)
 Variable A: Set.
 
-(** Generic definition of partial maps from identifiers to some type A *)
-Definition Map : Set := string -> option A.
+(** Generic definition of partial maps from identifiers to some type A
+    encoded as sorted lists of pairs *)
+Record Map : Set := mkMap {
+  data :> list (string * A); (* Maps can be coerced to their data field *)
+  correct : Sortedb _ (pair_ltb _) data = true;
+}.
+
+(* Note to the curious reader: <<Map>> is a dependently typed struct as
+   its <<correct>> field depends on its <<data>> field. So comparing two
+   instances of <<Map>> would require comparing proofs, which is notably
+   hard/impossible to do. However in this particular case, the proof is
+   simply an equality on booleans, which are equipped with a decidable
+   equality. In this case, it is known that we have `uniqueness of identify
+   proofs`, meaning that we won't have to compare anything, as there is a
+   single inhabitant of these types. This allows us to compare maps
+   just as if they were only simply typed lists *)
+
+
+(* A comes with a boolean equality *)
+Variable Aeqb : A -> A -> bool.
+Hypothesis Aeqb_eq: forall x y, Aeqb x y = true -> x = y.
+Hypothesis Aeqb_neq: forall x y, Aeqb x y = false -> x <> y.
+Hypothesis Aeqb_refl: forall x, Aeqb x x = true.
+
+(* Equality over pairs of string * A *)
+Definition pair_eq elt1 elt2 : bool :=
+  (((fst elt1) =? (fst elt2))%string &&
+   Aeqb (snd elt1) (snd elt2))%bool.
+
+(* begin hide *)
+Lemma pair_eq_eq: forall x y, pair_eq x y = true -> x = y.
+Proof.
+intros [k1 v1] [k2 v2] heq.
+apply andb_prop in heq as [h1 h2]; simpl in *.
+apply String.eqb_eq in h1 as ->.
+now apply Aeqb_eq in h2 as ->.
+Qed.
+
+Lemma pair_eq_neq: forall x y, pair_eq x y = false -> x <> y.
+Proof.
+intros [k1 v1] [k2 v2] hneq h; subst.
+injection h; intros; subst; clear h.
+apply Bool.andb_false_iff in hneq; simpl in *.
+destruct hneq as [h | h].
+- now apply String.eqb_neq in h.
+- now apply Aeqb_neq in h.
+Qed.
+
+Lemma pair_eq_refl: forall x, pair_eq x x = true.
+Proof.
+intros [k v]; unfold pair_eq; simpl.
+now rewrite Aeqb_refl, String.eqb_refl.
+Qed.
+(* begin hide *)
+
+(** Boolean equality on <<Map>>s *)
+(* As stated in the previous note, we only compare the underlying list,
+   because of the uniqueness of identity proofs.
+   Note that we also rely on the coercion from map to (data map) provided
+   by the system. The "full" statement should be
+   ``eqb _ pair_eq (data map1) (data map2)`` but this version is a bit 
+   more readable *)
+Definition eqb (map1 map2: Map) : bool :=
+  (eqb _ pair_eq map1 map2).
+
+Lemma eqb_eq: forall map1 map2, eqb map1 map2 = true -> map1 = map2.
+Proof.
+intros [l1 h1] [l2 h2] h; unfold eqb in h; simpl in *.
+apply List.eqb_eq in h as ->; [ | now apply pair_eq_eq].
+now rewrite (sorted_proof_unicity _ _ l2 _ h1 h2).
+Qed.
+
+Lemma eqb_neq: forall map1 map2, eqb map1 map2 = false -> map1 <> map2.
+Proof.
+intros [l1 h1] [l2 h2] hn h; unfold eqb in hn; simpl in *.
+injection h; clear h; intros; subst.
+rewrite List.eqb_refl in hn; [ discriminate | now apply pair_eq_refl].
+Qed.
 
 (** The empty map *)
-Definition empty: Map := fun _ => None.
+Definition empty: Map := mkMap nil (refl_equal _).
 
-(** Reading from a map, might return None *)
-Definition get_map (map: Map) id : option A := map id.
+(** Reading from a map, might return None if the key is not present *)
+Fixpoint get_map_ (map: list (string * A)) id : option A :=
+  match map with 
+  | nil => None
+  | (key, value) :: map =>
+      if (id =? key)%string
+      then Some value
+      else get_map_ map id
+end.
 
-(** Updating a binding in a map *)
-Definition set_map (map: Map) id (data: A) : Map := 
-    fun x => if String.eqb id x then Some data else get_map map x.
+(* wrapper around get_map_ *)
+Definition get_map (map: Map) key : option A := get_map_ map key.
 
-(** Removing a binding in a map *)
-Definition unset_map (map: Map) id : Map :=
-    fun x => if String.eqb id x then None else get_map map x.
+(** Updating a binding in a map: since we always keep our lists sorted,
+    we proceed by insertion sort, overriding the existing value if the 
+    key was already in use. *)
+Fixpoint insert_sorted (key: string) (value: A)
+  (l: list (string * A)) : list (string * A) :=
+  match l with
+  | [] => [(key, value)]
+  | (key', value') :: l' =>
+      if (key =? key')%string
+      then (key, value) :: l'
+      else if ltb key key'
+           then (key, value) :: l
+           else (key', value') :: insert_sorted key value l'
+  end.
+
+(* begin hide *)
+Lemma insert_sorted_hdrel: forall l key value,
+  HdRel (pair_lt _) (key, value) l ->
+  forall key' value',
+  ltb key key' = true ->
+  HdRel (pair_lt _) (key, value) (insert_sorted key' value' l).
+Proof.
+induction l as [ | [k v] data hi]; intros key value hhd key' value' hlt;
+    simpl in *; [now constructor | ].
+apply HdRel_inv in hhd; unfold pair_lt, pair_ltb in hhd; simpl in hhd.
+case_eq (String.eqb key' k); intro heq.
+- now constructor.
+- case_eq (ltb key' k); intro hk;  now constructor.
+Qed.
+
+Lemma insert_sorted_sorts: forall l, Sorted (pair_lt _) l ->
+  forall key value, Sorted (pair_lt _) (insert_sorted key value l).
+Proof.
+induction l as [ | [key value] data hi]; intros hsort key' value';
+    simpl in *; [ now repeat constructor | ].
+case_eq (String.eqb key' key); intro heq.
+- apply Sorted_inv in hsort as [ h0 h1].
+  constructor; [ assumption | ].
+  apply String.eqb_eq in heq; subst.
+  now apply HdRel_pair_lt_right with (value0 := value).
+- case_eq (ltb key' key); intro hkeys.
+  + constructor; [ assumption | ].
+    now constructor; unfold pair_lt; simpl.
+  + apply Sorted_inv in hsort as [ h0 h1].
+    constructor; [ now apply hi | ].
+    apply insert_sorted_hdrel;[ assumption | ].
+    apply String.eqb_neq in heq.
+    apply lt_ge in hkeys as [ h | h ]; [assumption | ].
+    now elim heq.
+Qed.
+
+Lemma insert_sorted_sorts_bool: forall l, Sortedb _ (pair_ltb _) l = true ->
+  forall key value, Sortedb _ (pair_ltb _) (insert_sorted key value l) = true.
+Proof.
+intros l h key value.
+apply reflect_Sorted in h; apply reflect_Sorted.
+now apply insert_sorted_sorts.
+Qed.
+(* begin hide *)
+
+(** Set a <<key>> to some <<value>> in a <<Map>>, overriding the existing
+    value if the <<key>> was already in use. *)
+Definition set_map (map: Map) key (value: A) : Map := 
+  let new_data := insert_sorted key value map in
+  mkMap new_data (insert_sorted_sorts_bool map (correct map) key value).
+
+(** Removing a key/value pair in a sorted list, based on the key.
+    Since we are stricly sorted, the first one (if any) is the only one *)
+Fixpoint remove_sorted (l: list (string * A)) id : list (string * A) :=
+  match l with 
+  | nil => nil
+  | (key, value) :: l =>
+      if (id =? key)%string
+      then l
+      else (key, value) :: remove_sorted l id
+end.
+
+(* begin hide *)
+Lemma remove_sorted_forall: forall l key value,
+  Forall (pair_lt _ (key, value)) l ->
+  forall key',
+  Forall (pair_lt _ (key, value)) (remove_sorted l key').
+Proof.
+induction l as [ | [key value] l hi]; intros k v hf key'; simpl in *;
+    [now constructor | ].
+case_eq (String.eqb key' key); intro heq; [ now apply Forall_inv_tail in hf | ].
+constructor; [now apply Forall_inv in hf | ].
+apply hi.
+now apply Forall_inv_tail in hf.
+Qed.
+
+Lemma remove_sorted_strongly_sorted: forall l,
+  StronglySorted (pair_lt _) l -> forall key,
+  StronglySorted (pair_lt _) (remove_sorted l key).
+Proof.
+induction 1 as [ | [key value] data hdata hi hforall ]; intros key';
+    simpl in *; [ now constructor | ].
+case_eq (String.eqb key' key); intro hk; [ assumption | ].
+constructor; [now apply hi | ].
+now apply remove_sorted_forall.
+Qed.
+
+Lemma remove_sorted_sorts: forall l, Sorted (pair_lt _) l ->
+  forall key, Sorted (pair_lt _) (remove_sorted l key).
+Proof.
+intros l hs k.
+apply StronglySorted_Sorted.
+apply remove_sorted_strongly_sorted.
+apply Sorted_StronglySorted; [| assumption].
+intros x y z.
+now apply pair_lt_trans.
+Qed.
+
+Lemma remove_sorted_sorts_bool: forall l, Sortedb _ (pair_ltb _) l = true ->
+  forall key, Sortedb _ (pair_ltb _) (remove_sorted l key) = true.
+Proof.
+intros l hs key.
+apply reflect_Sorted in hs; apply reflect_Sorted.
+now apply remove_sorted_sorts.
+Qed.
+(* end hide *)
+
+(** Remove an entry from a map. Once this function terminates, the <<key>>
+  is no longer mapped to anything in the map. *)
+Definition unset_map (map: Map) key : Map :=
+  let new_data := remove_sorted (data map) key in 
+  mkMap new_data (remove_sorted_sorts_bool (data map) (correct map) key).
+
+(** In this section, we proove that our maps enjoy the extensionality
+    property: it is enough to compare all keys to test the equality 
+    between maps.
+    This part reallies on the fact that our <<lt>> relation is transitive. *)
+Section Extensionality.
+
+(* If a <<key>> is less that all the keys in a list, then getting <<key>>
+   from the list will return nothing. *)
+Lemma get_lt_none: forall l key value, Forall (pair_lt _ (key, value)) l ->
+  get_map_ l key = None.
+Proof.
+induction l as [ | [k v] l hi]; intros key value hf; simpl in *; [reflexivity | ].
+case_eq (String.eqb key k); intro hk.
+- apply Forall_inv in hf.
+  unfold pair_lt, pair_ltb in hf; simpl in hf.
+  apply lt_not_eq in hf; rewrite hf in hk; discriminate.
+- apply Forall_inv_tail in hf.
+  now apply hi in hf.
+Qed.
+
+(* If two lists are strongly sorted, and all keys map to the same value (or 
+   absence of value, then they are equal. *)
+Lemma map_extensionality_: forall l1 l2,
+  StronglySorted (pair_lt _) l1 ->
+  StronglySorted (pair_lt _) l2 ->
+  (forall key, get_map_ l1 key = get_map_ l2 key) ->
+  l1 = l2.
+Proof.
+induction l1 as [ | [k1 v1] l1 hi]; intros [ | [k2 v2] l2] hs1 hs2 hk;
+    simpl in *.
+- reflexivity.
+- specialize hk with k2.
+  rewrite String.eqb_refl in hk.
+  discriminate hk.
+- specialize hk with k1.
+  rewrite String.eqb_refl in hk.
+  discriminate hk.
+- apply StronglySorted_inv in hs1 as [hs1 hf1].
+  apply StronglySorted_inv in hs2 as [hs2 hf2].
+  case_eq (String.eqb k1 k2); intro hk12.
+  + replace k2 with k1 in * by now apply String.eqb_eq in hk12.
+    rewrite (hi l2); intuition.
+    * replace v2 with v1; [ reflexivity | ].
+      specialize hk with k1.
+      rewrite String.eqb_refl in hk.
+      now injection hk.
+    * specialize hk with key.
+      case_eq (String.eqb key k1); intro heq; rewrite heq in hk; [| assumption].
+      apply String.eqb_eq in heq; subst.
+      now rewrite (get_lt_none l1 k1 v1), (get_lt_none l2 k1 v2).
+  + case_eq (ltb k1 k2); intro hcomp.
+    * specialize hk with k1.
+      rewrite String.eqb_refl, hk12 in hk.
+      rewrite (get_lt_none l2 k1 v1) in hk; [discriminate | ].
+      eapply Forall_pair_lt; [ | apply hf2].
+      now apply hcomp.
+    * specialize hk with k2.
+      rewrite String.eqb_sym in hk12.
+      rewrite String.eqb_refl, hk12 in hk.
+      rewrite (get_lt_none l1 k2 v2) in hk; [discriminate | ].
+      eapply Forall_pair_lt; [ | apply hf1].
+      unfold pair_lt, pair_ltb; simpl.
+      apply lt_ge in hcomp as [ ? | heq]; [assumption | ].
+      subst; rewrite String.eqb_refl in hk12; discriminate.
+Qed.
+ 
+(** If two maps have the exact same mappings, they are equal. *)
+Lemma map_extensionality: forall map1 map2,
+  (forall key, get_map map1 key = get_map map2 key) -> map1 = map2.
+Proof.
+intros map1 map2 hk.
+apply eqb_eq.
+destruct map1 as [l1 hl1]; destruct map2 as [l2 hl2];
+   unfold eqb, get_map in *; simpl in *.
+replace l2 with l1; [ now apply List.eqb_refl; apply pair_eq_refl | ].
+apply map_extensionality_; intuition.
+- apply Sorted_StronglySorted; [now intros x y z; apply pair_lt_trans | ].
+  now apply reflect_Sorted.
+- apply Sorted_StronglySorted; [now intros x y z; apply pair_lt_trans | ].
+  now apply reflect_Sorted.
+Qed.
+
+End Extensionality.
 
 Lemma get_set_map: forall map x y a,
   get_map (set_map map x a) y =
-  if  String.eqb x y then Some a else get_map map y.
+  if  (y =? x)%string then Some a else get_map map y.
 Proof.
-now  unfold set_map, get_map; simpl.
+intros [l hs] x y a; unfold set_map, get_map; simpl.
+induction l as [ | [k v] l hi]; simpl in *; [reflexivity | ].
+case_eq (String.eqb x k); intro hk; simpl.
+- case_eq (String.eqb y x); intro hyx; rewrite hyx in *; [reflexivity | ].
+  apply String.eqb_eq in hk as ->.
+  now rewrite hyx.
+- apply andb_prop in hs as [hs hhd].
+  case_eq (ltb x k); intro hlt; simpl.
+  + now case_eq (String.eqb y x); intro hyx; rewrite hyx in *.
+  + case_eq (String.eqb y x); intro hyx; rewrite hyx in *.
+    * apply String.eqb_eq in hyx; subst.
+      rewrite hk.
+      now apply hi.
+    * case_eq (String.eqb y k); intro hyk; [reflexivity | ].
+      now apply hi.
+Qed.
+
+(* Sorted insertion in a sorted list commutes if both keys are different *)
+Lemma set_set_diff_: forall map x y a b z,
+  (x =? y)%string = false ->
+  get_map_ (insert_sorted y b (insert_sorted x a map)) z =
+  get_map_ (insert_sorted x a (insert_sorted y b map)) z.
+Proof.
+induction map as [ | [key value] tl hi]; intros x y a b z hne; simpl in *.
+- rewrite hne, String.eqb_sym, hne.
+  case_eq (ltb y x); intro hlt.
+  + rewrite ltb_antisym in hlt.
+    unfold leb in hlt.
+    rewrite Bool.negb_orb in hlt.
+    apply andb_prop in hlt as [ h1 h2 ].
+    now apply Bool.negb_true_iff in h1 as ->.
+  + rewrite ltb_antisym in hlt.
+    unfold leb in hlt.
+    rewrite Bool.negb_orb in hlt.
+    apply Bool.andb_false_iff in hlt as [ h | h ].
+    * now apply Bool.negb_false_iff in h as ->.
+    * apply Bool.negb_false_iff in h. 
+      rewrite h in hne; discriminate.
+- case_eq (String.eqb x key); intro hxkey; simpl.
+  + apply String.eqb_eq in hxkey; subst.
+    rewrite String.eqb_sym, hne; simpl.
+    case_eq (ltb y key); intro hlt; simpl insert_sorted.
+    * rewrite hne, ltb_antisym; unfold leb.
+      now rewrite hlt, String.eqb_refl.
+    * now rewrite String.eqb_refl.
+  + case_eq (String.eqb y key); intro hykey.
+    * apply String.eqb_eq in hykey; subst.
+      case_eq (ltb x key); intro hlt; simpl insert_sorted.
+      -- rewrite String.eqb_sym, hne, String.eqb_refl, ltb_antisym.
+         now unfold leb; rewrite hlt; simpl.
+      -- now rewrite String.eqb_refl, hne, hlt.
+    * case_eq (ltb x key); intro hltx.
+      -- case_eq (ltb y key); intro hlty; simpl insert_sorted.
+         ++ rewrite String.eqb_sym, hne, hykey, hlty, hxkey, hltx.
+            case_eq (ltb y x); intro h.
+            ** now rewrite ltb_antisym; unfold leb; rewrite h.
+            ** now rewrite ltb_antisym; unfold leb; rewrite h,
+                 String.eqb_sym, hne.
+         ++ rewrite String.eqb_sym, hne, hykey, hlty, hxkey, hltx.
+            case_eq (ltb y x); intro h; [ | reflexivity ].
+            assert (hw: ltb y y = true);
+                  [ | now rewrite ltb_irrefl in hw; discriminate ].
+            apply (ltb_trans y x y); [ assumption | ].
+            apply (ltb_trans x key y); [ assumption | ].
+            now rewrite ltb_antisym; unfold leb; rewrite hlty, hykey.
+     -- case_eq (ltb y key); intro hlty; simpl insert_sorted.
+        ++ rewrite hykey, hne, hlty, hltx, hxkey.
+           case_eq (ltb x y); intro h; [| reflexivity ].
+            assert (hw: ltb x x = true);
+                  [ | now rewrite ltb_irrefl in hw; discriminate ].
+            apply (ltb_trans x y x); [ assumption | ].
+            apply (ltb_trans y key x); [ assumption | ].
+            now rewrite ltb_antisym; unfold leb; rewrite hltx, hxkey.
+        ++ rewrite hykey, hxkey, hlty, hltx.
+           simpl.
+           case_eq (String.eqb z key); [ reflexivity | intro h].
+           now apply hi.
+Qed.
+
+Lemma set_set_diff_map: forall map x y a b,
+  String.eqb x y = false ->
+  set_map (set_map map x a) y b =
+  set_map (set_map map y b) x a.
+Proof.
+intros map x y a b hne; apply map_extensionality; intros z.
+unfold set_map, get_map; simpl.
+now apply set_set_diff_.
 Qed.
 
 (** Intermediate "state", which will be used to track types or values
@@ -35,6 +469,7 @@ Record RawState0: Set := mkRawState0 {
     local: Map;
 }.
 
+(* Wrappers around their _map counter-part *)
 Definition Empty0 : RawState0 := mkRawState0 empty.
 
 Definition get0 s k := get_map (local s) k.
@@ -47,10 +482,19 @@ Definition unset0 st k :=
 
 Lemma get0_set0: forall s x y a,
   get0 (set0 s x a) y =
-  if  String.eqb x y then Some a else get0 s y.
+  if (y =? x)%string then Some a else get0 s y.
 Proof.
 intros s x y a; unfold set0, get0; simpl.
 now rewrite get_set_map.
+Qed.
+
+Lemma set0_set0_diff: forall s x y a b,
+  (x =? y)%string = false ->
+  set0 (set0 s x a) y b =
+  set0 (set0 s y b) x a.
+Proof.
+intros s x y a b hne; unfold set0, get0; simpl.
+now rewrite set_set_diff_map.
 Qed.
 
 End Map.
@@ -58,6 +502,10 @@ End Map.
 Section RawState.
 Variable A: Set.
 Variable B: Set.
+
+Variable Aeqb : A -> A -> bool.
+Hypothesis Aeqb_eq: forall x y, Aeqb x y = true -> x = y.
+Hypothesis Aeqb_refl: forall x, Aeqb x x = true.
 
 (** Main "state", which stores a <<RawState0>> plus additional information
 (like a list of the already checked/defined functions *)
@@ -78,9 +526,22 @@ Definition get_info (s: RawState) f := get_map _ (info s) f.
 
 Lemma get_set: forall s x y a,
   get (set s x a) y =
-  if  String.eqb x y then Some a else get s y.
+  if  (y =? x)%string then Some a else get s y.
+Proof.
 intros [s ?] x y a; simpl.
-unfold set, get, set0, get0; simpl.
-now rewrite get_set_map.
+unfold set, get; simpl state.
+now rewrite get0_set0.
 Qed.
+
+Lemma set_set_diff: forall s x y a b,
+  (x =? y)%string = false ->
+  set (set s x a) y b =
+  set (set s y b) x a.
+Proof.
+intros [s ?] x y a b h; simpl.
+unfold set, get.
+simpl state.
+now rewrite (set0_set0_diff _ _ Aeqb_eq Aeqb_refl).
+Qed.
+
 End RawState.
