docs/formal/python_semantic/Lib/List.v
@@ -1,0 +1,153 @@
+Require Import List Sorted.
+Import ListNotations.
+
+(** This file is an extension of the <<List>> library by adding some
+    boolean predicates to reflect existing propositional ones. *)
+
+(** * Boolean version of Sorted *)
+Section BooleanSorted.
+
+Variable A: Type.
+(* Generic relation. Will usually be instantiated with an order like <<lt>>.
+   If the following file, I'll refer to <<R x y>> as "x smaller than y". *)
+Variable R : A -> A -> bool.
+
+(* <<HdRel a l>> means that either <<l>> is empty, or <<a>> is "smaller" than
+   the head of <<l>> *)
+Fixpoint HdRelb (a: A) (l: list A) : bool :=
+  match l with
+  | nil => true 
+  | b :: _ => R a b
+end.
+
+(* A list is (weakly) sorted if any element is "smaller" than the next.
+   A list is strongly sorted if any element is "smaller" than any of the 
+   following ones in the list. *)
+Fixpoint Sortedb (l : list A) : bool :=
+  match l with
+  | nil => true
+  | hd :: tl => andb (Sortedb tl) (HdRelb hd tl)
+end.
+
+Lemma reflect_HdRel: forall l a,
+  @HdRel A (fun x y => R x y = true) a l <-> HdRelb a l = true.
+Proof.
+induction l as [ | hd tl hi]; intros a; split; intro h; simpl in *.
+- reflexivity.
+- now constructor.
+- now apply HdRel_inv in h.
+- now constructor.
+Qed.
+
+Lemma reflect_Sorted: forall l,
+  @Sorted A (fun x y => R x y = true) l <-> Sortedb l = true.
+Proof.
+induction l as [ | hd tl hi]; split; intro h; simpl in *.
+- reflexivity.
+- now constructor.
+- apply Sorted_inv in h as [h0 h1].
+  apply andb_true_intro.
+  split; [ now apply hi | ].
+  now apply reflect_HdRel.
+- apply andb_prop in h as [h0 h1].
+  constructor; [ now apply hi | ].
+  now apply reflect_HdRel.
+Qed.
+
+Lemma reflect_Sorted_false: forall l,
+  (~ @Sorted A (fun x y => R x y = true) l) <-> Sortedb l = false.
+Proof.
+intros l; split; intro h.
+- case_eq (Sortedb l); intro hs; [| reflexivity].
+  apply reflect_Sorted in hs.
+  now elim hs.
+- intro hs.
+  apply reflect_Sorted in hs.
+  rewrite hs in h; discriminate.
+Qed.
+
+End BooleanSorted.
+
+(* In this section we define a boolean equality on lists (as long as the
+   underlying type has one), by pair-wise comparing the elements of the lists.
+*)
+Section ListEq.
+Variable A: Type.
+Variable Aeqb : A -> A -> bool.
+(* We need some hypothesis on the underlying equaliy, like reflexivity, ... *)
+Hypothesis Aeqb_eq: forall x y, Aeqb x y = true -> x = y.
+Hypothesis Aeqb_neq: forall x y, Aeqb x y = false -> x <> y.
+Hypothesis Aeqb_refl: forall x, Aeqb x x = true.
+Hypothesis Aeqb_trans: forall x y z,
+  Aeqb x y = true -> Aeqb y z = true -> Aeqb x z = true.
+
+Fixpoint eqb (l1 l2: list A) : bool :=
+  match (l1, l2) with
+  | (nil, nil) => true
+  | (hd1 :: tl1, hd2 :: tl2) => (Aeqb hd1 hd2 && eqb tl1 tl2)%bool
+  | (_, _) => false
+end.
+
+Lemma eqb_eq: forall l1 l2, eqb l1 l2 = true -> l1 = l2.
+Proof.
+induction l1 as [ | hd1 tl1 hi]; intros [ | hd2 tl2] heq; simpl in *;
+    try discriminate; [reflexivity | ].
+apply andb_prop in heq as [h1 h2].
+apply Aeqb_eq in h1.
+apply hi in h2.
+now subst.
+Qed.
+
+Lemma eqb_neq: forall l1 l2, eqb l1 l2 = false -> l1 <> l2.
+Proof.
+induction l1 as [ | hd1 tl1 hi]; intros [ | hd2 tl2] heq h; simpl in *;
+    try discriminate.
+injection h; intros hhd htl; clear h; subst.
+apply Bool.andb_false_iff in heq as [hb | hb].
+- rewrite Aeqb_refl in hb; discriminate.
+- apply hi in hb.
+  now elim hb.
+Qed.
+
+Lemma eqb_refl: forall l, eqb l l = true.
+Proof.
+induction l as [ | hd tl hi]; simpl in *; [ reflexivity | ].
+now rewrite Aeqb_refl, hi.
+Qed.
+
+Lemma eqb_trans: forall x y z,
+  eqb x y = true -> eqb y z = true -> eqb x z = true.
+Proof.
+induction x as [ | x xs hi]; intros [ | y ys] [ | z zs] hxy hyz;
+    simpl in *; try discriminate; [reflexivity | ].
+apply andb_prop in hxy as [hxy hxys].
+apply andb_prop in hyz as [hyz hyzs].
+apply andb_true_intro; split.
+- now apply (Aeqb_trans x y z).
+- now apply (hi ys zs).
+Qed.
+
+End ListEq.
+
+Require Eqdep_dec.
+
+Section ListProofUnicity.
+Import Eqdep_dec.
+
+Variable A: Type.
+Variable R: A -> A -> bool.
+
+(* The unicity of proofs comes in handy when manipulating dependently typed
+   structures which embeds some proofs. This lemma means that any two
+   proofs of the fact that a list is sorted or not are equal. Since
+   we can write one, this means there is a single proof of that fact,
+   and so we can replace any proof by this witness, and avoid difficult
+   dependent rewrites *)
+Lemma sorted_proof_unicity: forall l b (P Q: @Sortedb _ R l = b), P = Q.
+Proof.
+intros l b P Q.
+apply eq_proofs_unicity.
+now intros [] []; intuition.
+Qed.
+
+End ListProofUnicity.
